theories/rust_typing/typing.v
@@ -1,4 +1,4 @@
-From refinedrust Require Export type int int_rules products references functions uninit box programs enum maybe_uninit alias_ptr existentials arrays value.
+From refinedrust Require Export type program_rules int int_rules products references functions uninit box programs enum maybe_uninit alias_ptr existentials arrays value.
 From refinedrust Require Export automation.
 
 Global Open Scope Z_scope.
